\begin{example}
Let us examine equation
\[
  y' = \frac{y^2 + 2 x y}{x^2} = \frac{y(y + 2x)}{x^2} = \frac{y(y/x) + 2)}{x}
  = \frac{y}{x} (\frac{y}{x} + 2) = g(y/x), x \neq y, x \neq 0
\]
and $g(s) = s(s + 2)$. Let $z(x) = \frac{y(x)}{x}$. If $y$ is solution of $y' =
g(s) = g(\frac{y}{x})$, then $z'(x) = \frac{y'(x) x - y(x)}{x^2} = \frac{1}{x}
(g(z(x)) - z(x)) = \frac{1}{x} (z(x) (z(x) + 2) - z(x))$, which solutions are
given by
\[
  \int^z (z (z + 2) - z) dz = \int^x \frac{1}{x} dx \Leftrightarrow
  \frac{1}{3} z^3 + \frac{1}{2} z^2 = \ln |x| + C \Leftrightarrow
\]
\[
  \frac{1}{3} (\frac{y(x)}{x})^3 + \frac{1}{2} (\frac{y(x)}{x})^2 = \ln |x| + C
\]
\end{example}
\begin{example}
Let us examine equation
\[
  y' = (x + y)^2 = f(ax + by + c), a = b = 1, c = 0
\]
and $f(z) = z^2$. Let $z(x) = x + y(x)$ and the separable equation is
\[
  z' = 1 + z^2 \Rightarrow \int^z 1 + z^2 dz = \int^x \frac{1}{x} dx, x \neq 0
\]
\[
  \Leftrightarrow \int^z \frac{1}{1 + z^2} dz = \int^x 1 dx
\]
\[
  \arctan(z) = x + C_0 \Leftrightarrow x + y = \tan x + C_1, C_1 = \tan C_0
  \Leftrightarrow y = \tan x - x + C_1
\]
\end{example}
