\begin{example}
Find all solutions of the differential equation given that $f(t) = e^{-t}$ is a
solution:
\begin{equation}
  f''(t) + 2 f'(t) + f(t) = 0
\end{equation}
\noindent\emph{Solution} 

Surely the solution $f(t) = e^{-t} > 0, \forall t \in \Re$. Let $f_2(t) = f_1(t) v(t)$.
\[
  f_2' = f_1' v + f_1 v'
\]
\[
  f_2'' = f_1'' v + f_1' v' + f_1' v' + f_1 v'' = f_1'' v + 2 f_1' v' + f_1 v''
\]
Now Equation (4) can be written as:
\begin{multline*}
  f_1'' v + 2 f_1'v' + f_1 v'' + 2 (f_1' v + f_1 v') + f_1 v = f_1 v'' + (2
  f_1' + 2 f_1 ) v' + (f_1'' + 2 f_1' + f_1) v = \\
  f_1 v'' + (2 f_1' + 2 f_1) v' = v'' + 2 \left(\frac{f_1' + f_1}{f_1}\right) v' = 0
\end{multline*}
Let $w = v'$:
\begin{multline*}
  w' + 2 \left(\frac{f_1' + f_1}{f_1}\right) w = 0 \Leftrightarrow w = e^{-2
  \int (\frac{f_1'}{f_1} + 1)} \Leftrightarrow \\ v = \int \left [ e^{-2 \int
  (\frac{f'}{f} + 1)} \right ] = \int (1 + C_1) = C_1 t + \frac{t^2}{2} + C_2,
  C_1, C_2 \in \Re
\end{multline*}
As $W(f_1, f_2) = v' f_1^2 = e^{-2 \int (\frac{f_1'}{f_1} + 1)} e^{-2t} \neq
0$, then $f_2(t) = e^{-t} \left [ C_1 t + \frac{t^2}{2} + C_2 \right ]$ is all
solutions for Equation (4).
\end{example}
